---
layout: post
title:  "A stroll through the Bayesian central limit theorem.  Part 2: The actual BCLT."
date:   2020-12-04 02:00:00 -0800
categories: bayes
---

In the previous post, I introduced some notation and concepts that I'll
now carry forward into an actual sketch of how to prove the BCLT.

# Re-write a posterior expectation as a random function that doesn't diverge.

Recall that, for the BCLT we need to analyze quantites of the following form:

$$
\mathbb{E}[\phi(\theta) | x] =
\frac{\int \phi(\theta) \exp(\sum_{n=1}^N \ell(x_n | \theta))p(\theta) d\theta}
     {\int \exp(\sum_{n=1}^N \ell(x_n | \theta))p(\theta) d\theta}.
$$

And recall that, to prove asymptotic normality of the MLE, we studied
the asymptotic behavior of the Taylor expansion of the
random log likelihood function,

$$
\theta \mapsto \frac{1}{N} \sum_{n=1}^N \ell(x_n \vert \theta).
$$

The factor of $$1/N$$ in the MLE is a stark difference with the Bayesian
case, as the posterior involves the random function

$$
\theta \mapsto \sum_{n=1}^N \ell(x_n | \theta),
$$

which diverges as $$N \rightarrow \infty$$!  Before even beginning, we must
re-write our expectation in a form involving something that looks like sample
averages, not a divergent sum.

To do so, we'll first form a Taylor series expansion.  For the moment, we'll
expand around a generic $$\bar\theta$$.

$$
\sum_{n=1}^N \ell(x_n | \theta) =
    \sum_{n=1}^N \ell(x_n | \bar\theta) +
    \sum_{n=1}^N \ell_{(1)}(x_n | \bar\theta)(\theta - \bar\theta) +
    \frac{1}{2}\sum_{n=1}^N \ell_{(2)}(x_n | \bar\theta)(\theta - \bar\theta)^2 +
    \frac{1}{6}\sum_{n=1}^N \ell_{(3)}(x_n | \tilde\theta)(\theta - \bar\theta)^3.
$$

Next, we'll re-parameterize our posterior.  We expect the posterior to
concentrate at rate $$\sqrt{N}$$.  So let's try a parameterization that inflates
$$\thet$$ at this scale.  Specifically, for any $$\bar\theta$$ depending only on
the data, we can define the Bayesian parameter

$$
\tau := \sqrt{N} (\theta - \bar\theta)
\quad\quad \Leftrightarrow \quad \quad
\theta = \frac{\tau}{\sqrt{N}} + \bar\theta.
$$

(The prior will transform so that $$p(\tau) d\tau = p(\theta) d\theta$$.)
